\documentclass[14pt]{article}
\usepackage[spanish]{babel}
\author{Brandon Rodriguez}
\title{Tarea 2}

\begin{document}

\maketitle
\section{Ejercicio 1}
 $ n^3  \geq  n^ 2 $
\\
\\
 \textbf{Caso Base}
\\
\\
$ 0^3 \geq 0^2 $
\\
$ 0 \geq 0 $
\\
\\
 \textbf{Inducción}
\\

Hipótesis Inductiva
\\
$ n^3  \geq  n^ 2 $
\\

Demostración
\\
$ (n+1)^3 \geq (n+1)^2 $
\\
$\frac { (n+1)(n^2+n+1)} {(n+1)} \geq \frac {(n+1)^2 } {(n+1)} $
\\
$ n^2+n+1 \geq n+1  $
\\
$ n^2+n+1-1 \geq n+1-1  $
\\
$ n^2+n \geq n  $
\\
$   n^2+n-n \geq n-n    $
\\
$$ n^2 \geq 0  $$
\\
\\
\\
\\
\\
\\
\\

\section{Ejercicio 2}

$\forall\ n.\ (1+x)^n\geq nx+1$
\\
\\
\textbf{Caso Base}
\\
$ (1+x)^0 \geq x(0)+1 $
\\
$ x \geq 1 $
\\
\\
\textbf{Inducción}
\\

Hipótesis Inductiva
\\
$\forall\ n.\ (1+x)^n\geq nx+1$
\\

Demostración 
\\ 
$(1+x)^n\geq nx+1$
\\
$(1+x)^n(x+1)\geq (nx+1)(x+1)$
\\
$(1+x)^{n+1}\geq (nx+1)(x+1)$
\\
$=1+(n+1)x+nx^2 \geq 0$
\\
$$(1+x)^{n+1}\geq 1+(n+1)x$$






\end{document}
\
\